Leansubst/Examples.lean
@@ -1,3 +1,132 @@
 import Leansubst.Basic
 
+/-- A simple lambda calculus with custom variable substitution operation. -/
+inductive Term where
+  | var : Nat →           Term -- Variable in de Bruijn index.
+  | app : Term → Term →   Term -- Function application.
+  | lam : String → Term → Term -- Function abstraction.
 
+def shift : Term → Nat → Nat → Term
+  | .var v,    n, m => if n <= v then .var (v + m) else .var v
+  | .app l r,  n, m => .app (shift l n m) (shift r n m)
+  | .lam x r,  n, m => .lam x (shift r (n + 1) m)
+
+def subst : Term → Nat → Term → Term
+  | .var v,    n, t => if n < v then .var (.pred v) else if n = v then shift t 0 n else .var v
+  | .app l r,  n, t => .app (subst l n t) (subst r n t)
+  | .lam x r,  n, t => .lam x (subst r (n + 1) t)
+
+/-!
+To use Leansubst v0.1, we need to map `Term` to `Leansubst.Expr`.
+This requires us to provide a signature.
+
+If your terms are defined in more than one mutually inductive types,
+it suffices to map everything into one single type `Leansubst.Expr` (as long as it is an injection).
+-/
+
+inductive Sig where
+  | var :          Sig
+  | app :          Sig
+  | lam : String → Sig
+
+def toExpr : Term → Leansubst.Expr Sig
+  | .var i   => .var i                              -- `var` must be mapped to `var` (no "fancy" variables).
+  | .app l r => .node .app     [toExpr l, toExpr r] -- `app` is a node with two children.
+  | .lam x r => .node (.lam x) [.binder (toExpr r)] -- `lam` is a node with one child "inside" a binder.
+
+open Leansubst
+
+abbrev Expr := Leansubst.Expr Sig
+abbrev Subst := Leansubst.Subst Sig
+
+/-!
+Now we prove that the mapping is an injection.
+This should be trivial (simply keep applying `injection`s).
+-/
+
+theorem to_expr_inj (s t : Term) : toExpr s = toExpr t → s = t := by
+  induction s generalizing t with
+  | var i =>
+    cases t <;> intros <;> try injections
+    rename_i h; rw [h]
+  | app l r ihl ihr =>
+    cases t <;> intros <;> try injections
+    rename_i l' r' h; injection h with _ h; injections h₁ _ h₂ _
+    congr; exacts [ihl _ h₁, ihr _ h₂]
+  | lam x r ih =>
+    cases t <;> intros <;> try injections
+    rename_i x' r' h; injection h with _ h; injections h₁ _ _ h₂
+    congr; exact ih _ h₂
+
+/-!
+And that our own substitution function agrees with `Leansubst.Subst.apply`.
+This can be much more involved... Currently I don't know how to automate this.
+-/
+
+theorem to_expr_shift (s : Term) (n m : Nat) :
+    toExpr (shift s n m) = Subst.apply (Subst.up n (Subst.shift _ m)) (toExpr s) := by
+  induction s generalizing n with
+  | var i =>
+    rw [shift]
+    split <;> simp only [toExpr, Subst.apply, Subst.apply.nested]
+    case inl h =>
+      have ⟨d, hd⟩ := Nat.le.dest h; subst hd; clear h
+      congr; simp [Subst.shift, Subst.up_get_high]
+      rw [Nat.add_comm n d, Nat.add_assoc, Nat.add_comm n m, Nat.add_assoc]
+    case inr h =>
+      congr; simp [Subst.shift, Subst.up_get_low _ _ _ (Nat.lt_of_not_le h)]
+  | app l r ihl ihr =>
+    simp only [toExpr, Subst.apply, Subst.apply.nested]
+    congr; exacts [ihl _, ihr _]
+  | lam x r ih =>
+    simp only [toExpr, Subst.apply, Subst.apply.nested]
+    congr; exacts [ih _]
+
+theorem to_expr_subst (s t : Term) (n : Nat) :
+    toExpr (subst s n t) = Subst.apply (Subst.single n (toExpr t)) (toExpr s) := by
+  induction s generalizing n with
+  | var i =>
+    rw [subst]
+    split <;> (try split) <;> simp only [subst, toExpr, Subst.single, Subst.apply, Subst.apply.nested]
+    case inl h =>
+      congr
+      cases i with
+      | zero => contradiction
+      | succ i =>
+        have ⟨d, hd⟩ := Nat.le.dest (Nat.le_of_lt_succ h); subst hd; clear h
+        rw [← Nat.add_succ, Subst.up_get_high]; simp
+        rw [Nat.add_succ, Nat.pred_succ]; simp [Subst.shift, Subst.apply, Subst.id]
+        rw [Nat.add_comm]
+    case inr.inl h₁ h₂ =>
+      subst h₂; clear h₁
+      conv => rhs; rhs; rw [← Nat.add_zero n]
+      rw [Subst.up_get_high, to_expr_shift, Subst.up]; simp
+    case inr.inr h₁ h₂ =>
+      have h := Nat.lt_of_le_of_ne (Nat.le_of_not_lt h₁) (Ne.symm h₂); clear h₁ h₂
+      rw [Subst.up_get_low _ _ _ h]
+  | app l r ihl ihr =>
+    simp only [subst, toExpr, Subst.single, Subst.apply, Subst.apply.nested]
+    congr; exacts [ihl _, ihr _]
+  | lam x r ih =>
+    simp only [subst, toExpr, Subst.single, Subst.apply, Subst.apply.nested]
+    congr; exacts [ih _]
+
+/-!
+Now we are finally ready to go!
+-/
+
+local notation t " ⟦" n:80 " ↟ " m:79 "⟧"  => shift t n m
+local notation t " ⟦" n:80 " ↦ " t':79 "⟧" => subst t n t'
+
+syntax "lsimp" : tactic
+macro_rules
+  | `(tactic| lsimp) =>
+    `(tactic| apply to_expr_inj; simp only [Subst.single, toExpr, to_expr_shift, to_expr_subst]; simp)
+
+theorem shift_shift_disjoint_ind (e k a b c) : e ⟦(b + k) ↟ c⟧ ⟦k ↟ a⟧ = e ⟦k ↟ a⟧ ⟦(a + b + k) ↟ c⟧ := by
+
+  lsimp
+
+example (s) : .lam "x" (.app (.var 0) (.var 3)) ⟦2 ↦ s⟧ = .lam "x" (.app (.var 0) (s ⟦0 ↟ 1⟧)) := by
+  lsimp
+  sorry
